crnf.v correction

crnf.v
@@ -1,7 +1,80 @@
 Require Export weak.
 Require Import cases.
 
-Definition is_crnf t r := is_rnf r /\ forall s, inf_beta t s -> is_rnf s -> red_wh t r /\ inf_wh r s.
+Inductive step_wh_n : nat -> term -> term -> Prop :=
+| step_wh_0 : forall t s, t == s -> step_wh_n 0 t s
+| step_wh_more : forall n t s s', step_wh t s -> step_wh_n n s s' -> step_wh_n (S n) t s'.
+
+Lemma lem_step_wh_n_morphism : forall n, morphism (step_wh_n n).
+Proof.
+  unfold morphism.
+  induction 1.
+  - pose_term_eq; ycrush.
+  - intros; econstructor.
+    + rewrite H1 in H; apply H.
+    + pose_term_eq; ycrush.
+Qed.
+
+Add Parametric Morphism (n : nat) : (step_wh_n n) with
+    signature term_eq ==> term_eq ==> iff as step_wh_n_mor.
+Proof.
+  split; intro; eapply lem_step_wh_n_morphism; pose_term_eq; eauto.
+Qed.
+
+Lemma lem_step_wh_n_to_red_wh : forall n t s, step_wh_n n t s -> red_wh t s.
+Proof.
+  induction 1; ycrush.
+Qed.
+
+Lemma lem_red_wh_to_step_wh_n : forall t s, red_wh t s -> exists n, step_wh_n n t s.
+Proof.
+  induction 1; ycrush.
+Qed.
+
+Lemma lem_step_wh_n_unique : forall n t s s', step_wh_n n t s -> step_wh_n n t s' -> s == s'.
+Proof.
+  induction n.
+  - pose_term_eq; iauto 2.
+  - intros t s s' H1 H2.
+    inversion_clear H1.
+    inversion_clear H2.
+    pose lem_step_wh_unique; ycrush.
+Qed.
+
+Lemma lem_step_wh_n_decompose :
+  forall m n t s s', step_wh_n n t s -> step_wh_n m t s' -> m >= n -> red_wh s s'.
+Proof.
+  induction m.
+  - scrush.
+  - intros.
+    inversion_clear H0.
+    assert (HH: (m = n - 1 /\ n > 0) \/ m >= n) by omega.
+    destruct HH.
+    + assert (m >= n - 1) by omega.
+      assert (step_wh_n (n - 1) s0 s).
+      inversion H; subst; sauto.
+      assert (HH1: s1 == s0) by
+	  Reconstr.reasy (@weak.lem_step_wh_unique) Reconstr.Empty.
+      rewrite HH1 in *; scrush.
+      ycrush.
+    + destruct n.
+      * assert (HH: t == s) by scrush.
+        rewrite HH in *; clear HH.
+        assert (red_wh s0 s') by
+	    Reconstr.reasy (@lem_step_wh_n_to_red_wh) Reconstr.Empty.
+        ycrush.
+      * assert (m >= n) by omega.
+        inversion_clear H.
+        assert (HH: s1 == s0) by
+	    Reconstr.reasy (@weak.lem_step_wh_unique) Reconstr.Empty.
+        rewrite HH in *; clear HH.
+        assert (red_wh s0 s') by
+	    Reconstr.reasy (@lem_step_wh_n_to_red_wh) Reconstr.Empty.
+        ycrush.
+Qed.
+
+Definition is_crnf t r := is_rnf r /\
+                          exists n, step_wh_n n t r /\ forall s m, step_wh_n m t s -> is_rnf s -> m >= n.
 Hint Unfold is_crnf.
 
 Lemma lem_crnf_exists : forall t, has_rnf t -> exists r, is_crnf t r.
@@ -13,20 +86,29 @@ Proof.
   clear H2; revert HH1.
   rename HH2 into H.
   induction H; intros.
-  - exists x; unfold is_crnf; split; intros; rewrite H in *; pose_red_wh; pose lem_inf_beta_to_inf_wh; ycrush.
+  - exists x; unfold is_crnf; split.
+    + ycrush.
+    + exists 0; split.
+      * pose_term_eq; ycrush.
+      * intros; omega.
   - generalize (is_rnf_dec x); intro Hd; destruct Hd as [ Hd | Hd ].
-    + exists x; unfold is_crnf; pose_red_wh; pose lem_inf_beta_to_inf_wh; ycrush.
+    + exists x; unfold is_crnf; split; [ auto | exists 0 ].
+      split; [ pose_term_eq; ycrush | intros; omega ].
     + unfold is_crnf in *.
       generalize (IHstar HH3 HH1); intro HH; destruct HH as [r [Hr1 Hr2]].
       exists r; split; eauto; intros.
-      generalize (lem_rnf_red_wh x s H2 H3); intro HH; destruct HH as [s' [H4 [H5 H6]]].
-      inversion_clear H5; subst.
-      * exfalso; rewrite H7 in *; ycrush.
-      * assert (Hy0: y0 == y) by reasy (@weak.lem_step_wh_unique) Reconstr.Empty.
-        rewrite Hy0 in *; clear Hy0.
-        assert (red_wh y s') by ycrush.
-        assert (inf_beta y s) by (pose_inf_wh; pose lem_inf_wh_to_inf_beta; ycrush).
-        pose_red_wh; ycrush.
+      destruct Hr2 as [n0 [Hr21 Hr22]].
+      exists (S n0).
+      split; [ econstructor; eauto | idtac ].
+      intros.
+      destruct H2.
+      * rewrite H2 in *; ycrush.
+      * assert (HH: s == y) by
+	    Reconstr.reasy (@weak.lem_step_wh_unique) Reconstr.Empty.
+        rewrite HH in *; clear HH.
+        assert (n >= n0).
+        apply Hr22 with (s := s'); eauto.
+        omega.
 Qed.
 
 Definition crnf0 t (p : has_rnf t) : { r | is_crnf t r }.
@@ -41,4 +123,44 @@ Lemma lem_crnf_is_crnf : forall t (p : has_rnf t), is_crnf t (crnf t p).
 Proof.
   intros; unfold crnf.
   destruct (crnf0 t p); sauto.
+Qed.
+
+Lemma lem_is_crnf_unique : forall t r r', is_crnf t r -> is_crnf t r' -> r == r'.
+Proof.
+  unfold is_crnf; sauto.
+  assert (n >= n0) by scrush.
+  assert (n0 >= n) by scrush.
+  assert (n0 = n) by omega.
+  pose lem_step_wh_n_unique; ycrush.
+Qed.
+
+Lemma lem_crnf_unique : forall t p p', crnf t p == crnf t p'.
+Proof.
+  pose lem_crnf_is_crnf; pose lem_is_crnf_unique; ycrush.
+Qed.
+
+Lemma lem_crnf_property :
+  forall t r, is_crnf t r -> forall s, inf_beta t s -> is_rnf s -> red_wh t r /\ inf_wh r s.
+Proof.
+  intros.
+  assert (exists s', is_rnf s' /\ red_wh t s' /\ inf_wh s' s) by
+      Reconstr.reasy (@weak.lem_rnf_red_wh) Reconstr.Empty.
+  unfold is_crnf in *; simp_hyps.
+  assert (exists m, step_wh_n m t s') by
+      Reconstr.reasy (@lem_red_wh_to_step_wh_n) Reconstr.Empty.
+  simp_hyps.
+  assert (m >= n) by scrush.
+  assert (red_wh r s') by
+      Reconstr.reasy (@lem_step_wh_n_decompose) Reconstr.Empty.
+  Reconstr.reasy (@weak.lem_red_wh_refl, @weak.lem_beta_redex_to_step_wh, @lem_step_wh_n_to_red_wh, @weak.lem_aux_wh_to_inf_wh, @weak.lem_step_beta_to_inf_wh, @weak.lem_step_wh_to_inf_wh, @weak.lem_red_wh_to_inf_wh, @weak.lem_inf_beta_to_inf_wh, @weak.lem_red_beta_to_inf_wh, @weak.lem_inf_wh_prepend, @weak.lem_step_wh_to_red_wh) Reconstr.Empty.
+Qed.
+
+Lemma lem_red_wh_to_crnf : forall t (p : has_rnf t), red_wh t (crnf t p).
+Proof.
+  pose lem_crnf_is_crnf; pose lem_step_wh_n_to_red_wh; ycrush.
+Qed.
+
+Lemma lem_red_beta_to_crnf : forall t (p : has_rnf t), red_beta t (crnf t p).
+Proof.
+  Reconstr.reasy (lem_red_wh_to_crnf, lem_red_wh_to_red_beta) Reconstr.Empty.
 Qed.
